Add wf condition on SkEnv.t

compose/Skeleton.v
@@ -27,6 +27,20 @@ Module SkEnv.
   (* TODO: Fix properly to cope with Ctypes.fundef *)
   Definition t := Genv.t (AST.fundef (option signature)) unit.
 
+  Inductive wf (skenv: t): Prop :=
+  | wf_intro
+    (SYMBDEF: forall
+        id blk
+        (SYMB: skenv.(Genv.find_symbol) id = Some blk)
+     ,
+       <<DEF: exists skd, skenv.(Genv.find_def) blk = Some skd>>)
+    (DEFSYMB: forall
+        blk skd
+        (DEF: skenv.(Genv.find_def) blk = Some skd)
+     ,
+       <<SYMB: exists id, skenv.(Genv.find_symbol) id = Some blk>>)
+  .
+
   (* Definition project F V (skenv: t) (fl: flesh F V): option (Genv.t F V). *)
   (*   admit "". *)
   (* Defined. *)
@@ -82,6 +96,35 @@ Module SkEnv.
         ,
           <<SMALL: skenv_proj.(Genv.find_def) blk = None>>)
   .
+
+  Lemma project_preserves_wf
+        skenv
+        (WF: wf skenv)
+        keep skenv_proj
+        (PROJ: project skenv keep skenv_proj)
+    :
+      <<WF: wf skenv_proj>>
+  .
+  Proof.
+    inv WF. inv PROJ.
+    econs; eauto.
+    - ii.
+      destruct (classic (keep id)).
+      + erewrite SYMBKEEP in *; eauto.
+        erewrite DEFKEEP; eauto.
+        apply Genv.find_invert_symbol; ss.
+      + erewrite SYMBDROP in *; eauto. ss.
+    - ii.
+      destruct (Genv.invert_symbol skenv blk) eqn:T; cycle 1.
+      { exploit DEFORPHAN; eauto. i; des. clarify. }
+      rename i into id.
+
+      exploit Genv.invert_find_symbol; eauto. intro TT.
+      destruct (classic (keep id)).
+      + esplits; eauto. erewrite SYMBKEEP; eauto.
+      + exploit DEFDROP; eauto. i; des.
+        exploit SYMBDEF; eauto. i; des. clarify.
+  Qed.
 
   (* Definition project (skenv: t) (ids: list ident): option SkEnv.t. *)
   (*   admit "". *)
